parseExtensions returns (extensions X option (binders X len_of_binders)).

src/tls/Extensions.fst
@@ -35,14 +35,6 @@ private type canFail (a:Type) =
 
 (* PRE-SHARED KEYS AND KEY EXCHANGES *) 
 
-type pskIdentity = PSK.preSharedKey * PSK.obfuscated_ticket_age
-
-noeq type psk = 
-  // this is the truncated PSK extension, without the list of binder tags.
-  | ClientPSK of list pskIdentity
-  // this is just an index in the client offer's PSK extension
-  | ServerPSK of UInt16.t 
-
 // SI: copied from HSM. Should be here in Extensions only. 
 // PSK binders, actually the truncated suffix of TLS 1.3 ClientHello
 // We statically enforce length requirements to ensure that formatting is total.
@@ -52,18 +44,32 @@ let binderListBytes bs = List.Tot.fold_left (fun a (b:binder) -> a @| Parse.vlby
 type binders = bs: list binder {let l = length (binderListBytes bs) in 33 <= l /\ l <= 65535} 
 let bindersBytes (bs:binders): bytes = Parse.vlbytes2 (binderListBytes bs)
 
-let parseBinderList (b:bytes) = 
-  let rec (aux: b:bytes -> binders -> Tot (result binders) (decreases (length b))) = fun b binders ->    
+type pskIdentity = PSK.preSharedKey * PSK.obfuscated_ticket_age
+
+noeq type psk = 
+  // client identities and binders length
+  | ClientPSK of (list pskIdentity) * nat
+  // this is just an index in the client offer's PSK extension
+  | ServerPSK of UInt16.t 
+
+#set-options "--lax"
+// Return (binders,list of the binders' lengths). 
+let parseBinderList (b:bytes) : Tot (result (binders * (list nat))) = 
+  let rec (aux: b:bytes -> (binders * list nat) -> Tot (result (binders * list nat)) (decreases (length b))) = fun b (binders,lens) ->    
     if length b > 0 then
-      if length b >= 5 then // SI: check ?
-	match vlsplit 1 b with // SI: check 1?
+      if length b >= 33 then 
+	match vlsplit 1 b with 
 	| Error z -> error "parseBinderList failed to parse a binder"
-	| Correct(binder,bytes) -> aux bytes (binders @ [binder]) // use List.Total.snoc
+	| Correct(binder,bytes) -> 
+	  // SI: use List.Total.snoc
+	  let binders',lens' = (binders @ [binder], lens @ [length binder]) in
+	  aux bytes (binders',lens')
       else error "parseBinderList: too few bytes"
-    else Correct binders in
+    else Correct (binders,lens) in
   match vlparse 2 b with 
-  | Correct b -> aux b []
+  | Correct b -> aux b ([],[])
   | Error z -> error "parseBinderList" 
+
 
 val pskiBytes : PSK.preSharedKey * UInt32.t -> Tot bytes
 let pskiBytes (i,ot) = (PSK.preSharedKeyBytes i) @| bytes_of_int 4 (UInt32.v ot)
@@ -71,11 +77,10 @@ let pskiBytes (i,ot) = (PSK.preSharedKeyBytes i) @| bytes_of_int 4 (UInt32.v ot)
 val pskBytes : psk -> Tot bytes 
 let pskBytes psk = 
   match psk with 
-  | ClientPSK ids ->
+  | ClientPSK (ids,_binderlen) -> // SI: we don't want to serialize binderlen, correct?
     let ids' = List.Tot.fold_left (fun acc pski -> acc @| pskiBytes pski) empty_bytes ids in
-    vlbytes 2 ids' 
+    (vlbytes 2 ids') 
   | ServerPSK sid -> bytes_of_int 2 (UInt16.v sid)
-
 
 // SI: parsing uint32 depends upon #ota=4 precondition
 let ota_is_4 (b:bytes) = 
@@ -83,7 +88,6 @@ let ota_is_4 (b:bytes) =
   | Error z -> False
   | Correct(_id,ota) -> length ota == 4 
   
-//val parsePskIdentity : b:bytes{let _,ota = vlsplit 2 b in length ota == 4}  -> result pskIdentity
 val parsePskIdentity : b:bytes{ota_is_4 b} -> result pskIdentity
 let parsePskIdentity b = 
 //  let id,ota = vlsplit 2 b in // SI: check vlsplit use 
@@ -93,6 +97,7 @@ let parsePskIdentity b =
     begin
       match PSK.parsePreSharedKey id with 
       | Correct(id) -> 
+	// SI: check ota_is_4
 	let ota = UInt32.uint_to_t (int_of_bytes ota) in
 	Correct (id,ota)
       | Error z -> error "parsePskIdentity"
@@ -113,9 +118,10 @@ let parsePskIdentities b =
       else error "parsePSKIdentities too few bytes"
     else Correct psks in
   match vlparse 2 b with
-  | Correct b -> aux b []
-  | Error z -> error "parsePskIdentities" 
-
+  | Correct b -> (
+    if (length b >=7) then aux b []
+    else error "parsePskIdentities: too short")
+  | Error z -> error "parsePskIdentities: failed to parse" 
 
 val client_psk_parse : bytes -> result (psk * option binders)
 let client_psk_parse b = 
@@ -126,10 +132,11 @@ let client_psk_parse b =
     match parsePskIdentities (vlbytes2 ids) with 
     | Correct ids -> (
 	match parseBinderList binders with
-	| Correct binders -> Correct (ClientPSK ids, Some binders)
+	| Correct (binders,their_lens) -> (
+	  let len = List.Tot.fold_left (fun len b -> len + b) 0 their_lens in 
+	  Correct (ClientPSK (ids, len), Some binders))
 	| Error z -> error "client_psk_parse_binders")
     | Error z -> error "client_psk_parse_ids")
-
 	
 val server_psk_parse : bytes -> psk 
 let server_psk_parse b = ServerPSK (UInt16.uint_to_t (int_of_bytes b))
@@ -139,6 +146,14 @@ let parse_psk role b =
   match role with 
   | Client -> client_psk_parse b
   | Server -> Correct (server_psk_parse b, None)
+
+val len_of_psk : psk -> nat
+let len_of_psk psk =
+  match psk with 
+  | ClientPSK(ids,len) -> len
+  | ServerPSK(t) -> 0
+  
+#reset-options
  
 
 // https://tlswg.github.io/tls13-spec/#rfc.section.4.2.8
@@ -348,7 +363,7 @@ noeq type extension =
   | E_supported_groups of list namedGroup (* M, AF *) (* RFC 7919 *)  
   | E_signature_algorithms of signatureSchemeList (* M, AF *) (* RFC 5246 *)
   | E_key_share of CommonDH.keyShare (* M, AF *)
-  | E_pre_shared_key of list psk (* M, AF *)
+  | E_pre_shared_key of psk (* M, AF *)
   | E_early_data of earlyDataIndication
   | E_supported_versions of protocol_versions   (* M, AF *) 
   | E_cookie of b:bytes {0 < length b /\ length b < 65536}  (* M *)
@@ -441,13 +456,13 @@ let rec extensionPayloadBytes = function
   | E_supported_groups l       -> namedGroupsBytes l  
   | E_signature_algorithms sha -> signatureSchemeListBytes sha
   | E_key_share ks             -> CommonDH.keyShareBytes ks
-  | E_pre_shared_key psk       -> admit() //PSK.preSharedKeyBytes psk //17-04-21 TODO parse/format the list with ota
+  | E_pre_shared_key psk       -> pskBytes psk 
   | E_early_data edi           -> earlyDataIndicationBytes edi
   | E_supported_versions vv    ->
     // Sending TLS 1.3 draft versions, as other implementations are doing
     vlbytes 1 (List.Tot.fold_left (fun acc v -> acc @| versionBytes_draft v) empty_bytes vv)
   | E_cookie c                 -> (lemma_repr_bytes_values (length c); vlbytes 2 c)
-  | E_psk_key_exchange_modes _ -> admit()
+  | E_psk_key_exchange_modes kex -> client_psk_kexes_bytes kex
   | E_extended_ms              -> empty_bytes
   | E_ec_point_format l        -> ecpfListBytes l
   | E_unknown_extension (_,b)  -> b
@@ -472,23 +487,30 @@ let noExtensions =
   lemma_repr_bytes_values (length (extensionListBytes [])); 
   []
 
-val extensionsBytes: extensions -> b:bytes { length b < 2 + 65536 }
-let extensionsBytes exts =
-  let b = extensionListBytes exts in
-  lemma_repr_bytes_values (length b);
-  vlbytes 2 b
-
+#set-options "--lax"
 // SI: add a $delta$ param for truncated binders length. 
 // The main exported extensionBytes function will have _trunc's type. 
 // SI: move vlbytes_trunc to Format
 val vlbytes_trunc: lSize:nat -> b:bytes -> binderSize:nat -> Tot (r:bytes{length r = lSize + (length b) + binderSize})
 let vlbytes_trunc lSize b bSize = 
   bytes_of_int lSize ((length b) + bSize) @| b 
-  
-val extensionsBytes_trunc: extensions -> bindersSize:nat -> b:bytes { length b < 2 + 65536 } 
-let extensionsBytes_trunc exts delta = 
-  let exts = extensionsBytes exts in
-  vlbytes_trunc 2 exts delta 
+
+// old proposal 
+(* val extensionsBytes_trunc: extensions -> bindersSize:nat -> b:bytes { length b < 2 + 65536 }  *)
+(* let extensionsBytes_trunc exts delta =  *)
+(*   let exts = extensionsBytes exts in *)
+(*   vlbytes_trunc 2 exts delta  *)
+
+// SI: serialize, but pretend the len includes the binder_len. 
+// (we get the binder_len by looking it up in the E_pre_shared_key's payload.) 
+val extensionsBytes: extensions -> b:bytes { length b < 2 + 65536 }
+let extensionsBytes exts =
+  let b = extensionListBytes exts in
+  let binder_len = admit() in // SI: fixme 
+  lemma_repr_bytes_values (length b);
+  vlbytes_trunc 2 b binder_len
+
+#reset-options
 
 (*************************************************
  Extension parsing
@@ -526,7 +548,11 @@ let parseEcpfList b =
 
 (* We don't care about duplicates, not formally excluded. *)
 #set-options "--lax"
-val parseExtension: role -> bytes -> result extension
+
+let normallyNone ctor r =
+    (ctor r, None)
+
+val parseExtension: role -> bytes -> result (extension * option (binders * nat))
 let parseExtension role b =
   if length b < 4 then error "extension type: not enough bytes" else 
   let head, payload = split b 2 in
@@ -534,52 +560,65 @@ let parseExtension role b =
   | Error (_,s) -> error ("extension: "^s)
   | Correct data -> ( 
     match cbyte2 head with
-    | (0x00z, 0x00z) -> mapResult E_server_name (parseServerName role data)
+    | (0x00z, 0x00z) -> 
+//      mapResult E_server_name (parseServerName role data)
+      mapResult (normallyNone E_server_name) (parseServerName role data)
     | (0x00z, 0x0Az) -> // supported groups
       if length data < 2 || length data >= 65538 then error "supported groups" else
-      mapResult E_supported_groups (Parse.parseNamedGroups data)
+      mapResult (normallyNone E_supported_groups) (Parse.parseNamedGroups data)
 
     | (0x00z, 0x0Dz) -> // sigAlgs
       if length data < 2 ||  length data >= 65538 then error "supported signature algorithms" else 
-      mapResult E_signature_algorithms (TLSConstants.parseSignatureSchemeList data)
+      mapResult (normallyNone E_signature_algorithms) (TLSConstants.parseSignatureSchemeList data)
       
-    | (0x00z, 0x28z) -> mapResult E_key_share (CommonDH.parseKeyShare (Client? role) data)
+    | (0x00z, 0x28z) -> 
+      mapResult (normallyNone E_key_share) (CommonDH.parseKeyShare (Client? role) data)
 
-    | (0x00z, 0x29z) -> // head TBD, PSK
-      if length data < 2 then error "PSK" else 
-      mapResult E_pre_shared_key (admit()) (* 17-04-21 TODO PSK.parsePreSharedKey data *) 
+    | (0x00z, 0x29z) -> // PSK
+      if length data < 2 then error "PSK" else (
+      match parse_psk role data with
+      | Error z -> Error z
+      | Correct (psk,None) -> Correct (E_pre_shared_key psk, None)
+      | Correct (psk,Some binders) -> (
+	let len = len_of_psk psk in 
+	Correct (E_pre_shared_key psk, Some (binders,len))))
+      // mapResult E_pre_shared_key (parse_psk role data)
 
     | (0x00z, 0x2az) ->
       if length data <> 0 && length data <> 4 then error "early data indication" else
-      mapResult E_early_data (parseEarlyDataIndication data)
+      mapResult (normallyNone E_early_data) (parseEarlyDataIndication data)
+
     | (0x00z, 0x2bz) ->
       if length data <= 2 || length data >= 256 then error "supported versions" else
-      mapResult E_supported_versions (parseSupportedVersions data)
+      mapResult (normallyNone E_supported_versions) (parseSupportedVersions data)
 
     | (0xffz, 0x2cz) -> // cookie
       if length data <= 2 || length data >= 65538 then error "cookie" else
-      Correct (E_cookie data)
+      Correct (E_cookie data,None)
       
-    (* ToDo: | E_psk_key_exchange_modes _ *)
+    | (0x00z, 0x2dz) -> // key ex
+      if length data < 2 then error "psk_key_exchange_modes" else 
+      mapResult (normallyNone E_psk_key_exchange_modes) (parse_client_psk_kexes data)
 
     | (0x00z, 0x17z) -> // extended ms
       if length data > 0 then error "extended master secret" else 
-      Correct E_extended_ms
+      Correct (E_extended_ms,None)
       
     | (0x00z, 0x0Bz) -> // ec point format
       if length data < 1 || length data >= 256 then error "ec point format" else (
       lemma_repr_bytes_values (length data);
       match vlparse 1 data with
       | Error z -> Error z
-      | Correct ecpfs -> mapResult E_ec_point_format (parseEcpfList ecpfs))
+      | Correct ecpfs -> mapResult (normallyNone E_ec_point_format) (parseEcpfList ecpfs))
       
-    | _ -> Correct (E_unknown_extension (head,data)))
+    | _ -> Correct (E_unknown_extension (head,data),None))
 
 //17-05-08 TODO precondition on bytes to prove length subtyping on the result
-val parseExtensions: role -> b:bytes -> result extensions
+// SI: simplify binder accumulation code. (Binders should be the last in the list.)
+val parseExtensions: role -> b:bytes -> result (extensions * option (binders * nat))
 let parseExtensions role b =
   let rec aux: 
-    b:bytes -> list extension -> Tot (result (list extension)) (decreases (length b)) = fun b exts ->
+    b:bytes -> list extension * option (binders * nat) -> Tot (result (list extension * option (binders * nat))) (decreases (length b)) = fun b (exts,obinders) ->
     if length b >= 4 then
       let ht, b = split b 2 in
       match vlsplit 2 b with
@@ -587,19 +626,24 @@ let parseExtensions role b =
       | Correct(ext, bytes) -> (
 	(* assume (Prims.precedes (Prims.LexCons b) (Prims.LexCons (ht @| vlbytes 2 ext))); *)
 	match parseExtension role (ht @| vlbytes 2 ext) with
-	| Correct ext ->
+	// SI: 
+	| Correct (ext, Some binders) ->
 	  (match addOnce ext exts with // fails if the extension already is in the list
-	  | Correct exts -> aux bytes exts
+	  | Correct exts -> aux bytes (exts, Some binders) // keep the binder we got
 	  | Error z -> Error z)
+	| Correct (ext, None) ->
+	  (match addOnce ext exts with // fails if the extension already is in the list
+	  | Correct exts -> aux bytes (exts, obinders)  // use binder-so-far.
+	  | Error z -> Error z)	  
 	| Error z -> Error z)
-    else Correct exts in
+    else Correct (exts,obinders) in
   if length b < 2 then error "extensions" else
   match vlparse 2 b with
-  | Correct b -> aux b []
+  | Correct b -> aux b ([],None)
   | Error z -> error "extensions" 
 
 (* SI: API. Called by HandshakeMessages. *)
-val parseOptExtensions: r:role -> data:bytes -> result (option (list extension))
+val parseOptExtensions: r:role -> data:bytes -> result (option (list extension * option (binders * nat)))
 let parseOptExtensions r data =
   if length data = 0 
   then Correct None
